rename var + algo 4 colors

3_dutch_flag.dfy
@@ -9,37 +9,37 @@ method DutchFlag(a: array<Color>)
   ensures forall i,j :: 0 <= i < j < a.Length ==> Below(a[i],a[j])
   ensures multiset(a[..]) == multiset(old(a[..]))
 {
-  var r, w, b:= 0, 0, a.Length;
-  while w < b
-    invariant 0 <= r <= w <= b <= a.Length
-    invariant forall i:: 0 <= i < r ==> a[i] == Red
-    invariant forall i:: r <= i < w ==> a[i] == White
+  var i1, i2, b:= 0, 0, a.Length;
+  while i2 < b
+    invariant 0 <= i1 <= i2 <= b <= a.Length
+    invariant forall i:: 0 <= i < i1 ==> a[i] == Red
+    invariant forall i:: i1 <= i < i2 ==> a[i] == White
     invariant forall i:: b <= i < a.Length ==> a[i] == Blue
     invariant multiset(a[..]) == multiset(old(a[..]))
-    decreases  b - w
+    decreases  b - i2
   {
-    match a[w]
+    match a[i2]
     {
       case Red => 
-        a[r], a[w] := a[w], a[r];
-        r, w := r + 1, w + 1;
+        a[i1], a[i2] := a[i2], a[i1];
+        i1, i2 := i1 + 1, i2 + 1;
       case White => 
-        w := w + 1;
+        i2 := i2 + 1;
       case Blue => 
         b := b - 1;
-        a[w], a[b] := a[b], a[w];
+        a[i2], a[b] := a[b], a[i2];
     }
   }
 }
 
-predicate boolSorted(a:bool, b:bool)
+predicate boolBelow(a:bool, b:bool)
 {
   a == false || b == true // ff ft tt tf
 }
 
 method boolSort(a: array<bool>)
 modifies a
-ensures forall i,j:: 0 <= i < j < a.Length ==> boolSorted(a[i], a[j])
+ensures forall i,j:: 0 <= i < j < a.Length ==> boolBelow(a[i], a[j])
 ensures multiset(a[..]) == multiset(old(a[..]))
 {
   var f, t := 0, a.Length;
@@ -57,4 +57,45 @@ ensures multiset(a[..]) == multiset(old(a[..]))
       f := f+1;
     }  
   }
+}
+
+datatype quadriColors = C1 | C2 | C3 | C4
+
+predicate quadBelow(a: quadriColors, b: quadriColors)
+{
+  a == C1 || b == C4 || a == b || (b == C3 && a != C4)
+}
+
+method quadriFlag(a: array<quadriColors>) 
+modifies a
+ensures forall i,j :: 0 <= i < j < a.Length ==> quadBelow(a[i], a[j]);
+ensures multiset(a[..]) == multiset(old(a[..]))
+{
+  var i1, i2, i3, i4 := 0, 0, 0, a.Length;
+  while i3 < i4
+    invariant 0 <= i1 <= i2 <= i3 <= i4 <= a.Length
+    invariant forall i :: 0 <= i < i1 ==> a[i] == C1
+    invariant forall i :: i1 <= i < i2 ==> a[i] == C2
+    invariant forall i :: i2 <= i < i3 ==> a[i] == C3
+    invariant forall i :: i4 <= i < a.Length ==> a[i] == C4
+    invariant multiset(a[..]) == multiset(old(a[..]))
+    decreases  i4 - i3
+  {
+      match a[i3]
+        {
+          case C3 => 
+          i3 := i3 + 1;
+          case C1 =>  
+          a[i2], a[i3] := a[i3], a[i2];
+          a[i1], a[i2] := a[i2], a[i1];
+          i1, i2, i3  := i1+1, i2+1, i3+1;
+          case C2 =>
+          a[i2], a[i3] := a[i3], a[i2];
+          i2, i3 := i2+1, i3+1;
+          case C4 =>
+          i4 := i4 -1;
+          a[i4], a[i3] := a[i3], a[i4];
+        }
+    }
+  
 }
